save latest using service correspondence

working/composition/event_based_refinement/load_balancer/service_correspondence/addition_service/AdditionServiceSpec.t.dfy
@@ -3,26 +3,27 @@ include "../shared/AbstractServiceSpec.t.dfy"
 module AdditionServiceSpec refines AbstractServiceSpec {
     datatype Constants = Constants
 
-    datatype ServiceRequest = AddRequest(clientId: nat, seqNo: nat, x: int, y: int)
-    datatype ServiceReply = AddReply(clientId: nat, seqNo: nat, sum: int)
+    datatype ServiceRequest = AddRequest(seqNo: nat, x: int, y: int)
+    datatype ServiceReply = AddReply(seqNo: nat, sum: int)
 
-    datatype Variables = Variables(requests: set<ServiceRequest>, replies: set<ServiceReply>)
+    datatype Variables = Variables(requests: set<Message<ServiceRequest>>, replies: set<Message<ServiceReply>>)
 
     ghost predicate Init(c: Constants, v: Variables) {
         && |v.requests| == 0
         && |v.replies| == 0
     }
 
-    ghost predicate Add(c: Constants, v: Variables, v': Variables, requests: set<ServiceRequest>, replies: set<ServiceReply>) {
+    ghost predicate Add(c: Constants, v: Variables, v': Variables, requests: set<Message<ServiceRequest>>, replies: set<Message<ServiceReply>>) {
         exists request, reply ::
             && requests == {request} 
             && replies == {reply}
             && v'.requests == v.requests + {request}
             && v'.replies == v.replies + {reply}
-            && reply == AddReply(request.clientId, request.seqNo, request.x + request.y)
+            && reply.msg == AddReply(request.msg.seqNo, request.msg.x + request.msg.y)
+            && reply.dest == request.src
     }
 
-    ghost predicate Next(c: Constants, v: Variables, v': Variables, requests: set<ServiceRequest>, replies: set<ServiceReply>) {
+    ghost predicate Next(c: Constants, v: Variables, v': Variables, requests: set<Message<ServiceRequest>>, replies: set<Message<ServiceReply>>) {
         || Add(c, v, v', requests, replies)
     }
 
@@ -31,15 +32,17 @@ module AdditionServiceSpec refines AbstractServiceSpec {
     // (1) any packets on the network of type ServiceReply were actualy sent by this service (and correspondingly for requests received by this service). 
     // - this seems like it is an inductive invariant over distributed executions in our system model? and so it can be factored out
     // (2) inductive invariants over executions of the service itself (i.e., replies must contain the sum of a corresponding request)
-    lemma ServiceCorrespondence_NaiveVersion(sentPackets: set<seq<byte>>) 
+    lemma ServiceCorrespondence_NaiveVersion(sentPackets: set<Message<seq<byte>>>) 
         ensures forall pkt :: 
             && pkt in sentPackets
-            && ParseServiceReply(pkt).Some? ==>
-                exists v: Variables, request: ServiceRequest :: 
-                && ParseServiceReply(pkt).value in v.replies // this is (1)
+            && ParseServiceReply(pkt.msg).Some? ==>
+                exists v: Variables, request: Message<ServiceRequest> :: 
+                && Message(pkt.src, pkt.dest, ParseServiceReply(pkt.msg).value) in v.replies // this is (1)
                 && request in v.requests 
-                && ParseServiceReply(pkt).value == AddReply(request.clientId, request.seqNo, request.x + request.y) // this is (2)
-        ensures forall v: Variables, request: ServiceRequest ::
+                && ParseServiceReply(pkt.msg).value == AddReply(request.msg.seqNo, request.msg.x + request.msg.y) // this is (2)
+                && request.src == pkt.dest
+                && request.dest == pkt.src
+        ensures forall v: Variables, request: Message<ServiceRequest> ::
             && request in v.requests ==>
-            && MarshallServiceRequest(request) in sentPackets // this is (1)
+            && Message(request.src, request.dest, MarshallServiceRequest(request.msg)) in sentPackets // this is (1)
 }
