working/composition/event_based_refinement/load_balancer/service_correspondence/multiplication_service/MultiplicationServiceComponent.v.dfy
@@ -24,21 +24,62 @@ module MultiplicationServiceComponent refines RefinementTheorem {
         Host.Spec.Variables(v.hosts[0].requests, v.hosts[0].replies)
     }
 
-    ghost predicate InductiveMultiplication(c: Constants, v: Variables, req: Host.Spec.ServiceRequest)
+    ghost predicate Inv_InductiveMultiplicationImpl(c: Constants, v: Variables, req: Message<Host.Spec.ServiceRequest>)
         requires v.WF(c)
-        requires req in v.hosts[0].intermediateResults && |v.hosts[0].intermediateResults[req]| > 0
+        requires req in v.hosts[0].intermediateResults
+        requires |v.hosts[0].intermediateResults[req]| > 0
     {
         var latestResultIdx := |v.hosts[0].intermediateResults[req]| - 1;
-        v.hosts[0].intermediateResults[req][latestResultIdx].sum == (latestResultIdx + 1) * req.y
+        && v.hosts[0].intermediateResults[req][latestResultIdx].msg.sum == (latestResultIdx + 1) * req.msg.y
+        && v.hosts[0].intermediateResults[req][latestResultIdx].msg.seqNo == v.hosts[0].firstSeqNo[req] + (latestResultIdx)
+    }
+
+    ghost predicate Inv_InductiveMultiplication(c: Constants, v: Variables)
+        requires v.WF(c)
+    {
+        forall req :: 
+            && req in v.hosts[0].intermediateResults 
+            && |v.hosts[0].intermediateResults[req]| > 0 ==>
+            Inv_InductiveMultiplicationImpl(c, v, req)
+    }
+
+    lemma Inv_InductiveMultiplicationLemma(a: int, b: int, r: int)
+        requires r == a * b + b
+        ensures r == (a + 1) * b
+    {}
+
+    ghost predicate Inv_AddRequestsImpl(c: Constants, v: Variables, req: Message<AddSvc.ServiceRequest>)
+        requires v.WF(c)
+        requires req.src == c.hosts[0].idSelf
+        requires Message(req.src, req.dest, AddSvc.MarshallServiceRequest(req.msg)) in v.network.sentMsgs
+        requires req.msg.seqNo in v.hosts[0].seqNoAssgn
+    {
+        var multReq := v.hosts[0].seqNoAssgn[req.msg.seqNo];
+        var latestResultIdx := |v.hosts[0].intermediateResults[multReq]| - 1;
+        if latestResultIdx >= 0
+        then
+            if (req.msg.seqNo == v.hosts[0].intermediateResults[multReq][latestResultIdx].msg.seqNo + 1)
+            then req.msg == AddSvc.AddRequest(v.hosts[0].intermediateResults[multReq][latestResultIdx].msg.seqNo + 1, v.hosts[0].intermediateResults[multReq][latestResultIdx].msg.sum, multReq.msg.y)
+            else true
+        else 
+            req.msg == AddSvc.AddRequest(v.hosts[0].firstSeqNo[multReq], 0, multReq.msg.y)
+    }
+
+    ghost predicate Inv_AddRequests(c: Constants, v: Variables)
+        requires v.WF(c)
+    {
+        forall addReq : Message<AddSvc.ServiceRequest> :: 
+            && addReq.src == c.hosts[0].idSelf
+            && Message(addReq.src, addReq.dest, AddSvc.MarshallServiceRequest(addReq.msg)) in v.network.sentMsgs
+            && addReq.msg.seqNo in v.hosts[0].seqNoAssgn ==>
+            Inv_AddRequestsImpl(c, v, addReq)
     }
 
     ghost predicate Inv(c: Constants, v: Variables)
     {
         && v.WF(c)
-        && (forall req :: 
-            && req in v.hosts[0].intermediateResults 
-            && |v.hosts[0].intermediateResults[req]| > 0 ==>
-            InductiveMultiplication(c, v, req))
+        && Inv_InductiveMultiplication(c, v)
+        && Inv_AddRequests(c, v)
     }
 
     lemma RefinementInit(c: Constants, v: Variables)
@@ -55,41 +96,115 @@ module MultiplicationServiceComponent refines RefinementTheorem {
     {
         assume false;
     }
-
-    lemma InvHelper(c: Constants, v: Variables, v': Variables, msgOps: MessageOps, svcReply: AddSvc.ServiceReply)
+    
+    lemma ApplyServiceCorrespondence(c: Constants, v: Variables, v': Variables, msgOps: MessageOps, svcReply: Message<AddSvc.ServiceReply>) 
+        returns (addReq: Message<AddSvc.ServiceRequest>)
         requires Next(c, v, v', msgOps)
         requires Inv(c, v)
         requires Host.ReceiveIntermediateResponseImpl(c.hosts[0], v.hosts[0], v'.hosts[0], msgOps, svcReply) || Host.ReceiveFinalResponseImpl(c.hosts[0], v.hosts[0], v'.hosts[0], msgOps, svcReply)
-        ensures Inv(c, v')
+        ensures Message(addReq.src, addReq.dest, AddSvc.MarshallServiceRequest(addReq.msg)) in v.network.sentMsgs
+        ensures svcReply == Message(addReq.dest, addReq.src, AddSvc.AddReply(addReq.msg.seqNo, addReq.msg.x + addReq.msg.y))
+        // ensures svcReply.msg.sum == addReq.msg.x + addReq.msg.y
+        // ensures svcReply.msg.seqNo == addReq.msg.seqNo
+        // ensures svcReply.src == addReq.dest
+        // ensures svcReply.dest == svcReply.src
     {
-        var seqNo := svcReply.seqNo;
-
-        var multReq := v'.hosts[0].seqNoAssgn[seqNo];
-        assert v'.hosts[0].intermediateResults[multReq] == v.hosts[0].intermediateResults[multReq] + [svcReply];
         // apply inductive invariants from addition service
         AddSvc.ServiceCorrespondence_NaiveVersion(v.network.sentMsgs);
-        assert AddSvc.MarshallServiceReply(svcReply) in v.network.sentMsgs;
-        assert msgOps.recv == {AddSvc.MarshallServiceReply(svcReply)};
+        var pkt := Message(svcReply.src, svcReply.dest, AddSvc.MarshallServiceReply(svcReply.msg));
+        assert pkt in v.network.sentMsgs;
+        assert msgOps.recv == {pkt};
         AddSvc.MarshallParseInverse();
-        var v_add: AddSvc.Variables, request: AddSvc.ServiceRequest :| 
-            && AddSvc.ParseServiceReply(AddSvc.MarshallServiceReply(svcReply)).value in v_add.replies
+        assert AddSvc.ParseServiceReply(pkt.msg).value == svcReply.msg;
+        var v_add: AddSvc.Variables, request: Message<AddSvc.ServiceRequest> :| 
+            && Message(svcReply.src, svcReply.dest, AddSvc.ParseServiceReply(pkt.msg).value) in v_add.replies
             && request in v_add.requests 
-            && AddSvc.ParseServiceReply(AddSvc.MarshallServiceReply(svcReply)).value == AddSvc.AddReply(request.clientId, request.seqNo, request.x + request.y);
-        assert svcReply.sum == request.x + request.y;
+            && AddSvc.ParseServiceReply(pkt.msg).value == AddSvc.AddReply(request.msg.seqNo, request.msg.x + request.msg.y)
+            && request.src == pkt.dest
+            && request.dest == pkt.src;
+        addReq := request;
+        assert addReq in v_add.requests;
+        assert Message(addReq.src, addReq.dest, AddSvc.MarshallServiceRequest(addReq.msg)) in v.network.sentMsgs;
+        assert svcReply == Message(addReq.dest, addReq.src, AddSvc.AddReply(addReq.msg.seqNo, addReq.msg.x + addReq.msg.y));
+    }
 
-        // todo - this should follow from:
-        // (1) the inductive hypothesis 
-        // (2) knowledge that only a given host will send messages containing its client id (this maybe needs a stronger system model?)
-        assume request == AddSvc.AddRequest(c.hosts[0].id, seqNo, |v.hosts[0].intermediateResults[multReq]| * multReq.y, multReq.y);
+    lemma ApplyInv_AddRequestsImpl(c: Constants, v: Variables, addReq: Message<AddSvc.ServiceRequest>, multReq: Message<Host.Spec.ServiceRequest>, latestResultIdx: int)
+        requires Inv(c, v)
+        requires addReq.src == c.hosts[0].idSelf
+        requires Message(addReq.src, addReq.dest, AddSvc.MarshallServiceRequest(addReq.msg)) in v.network.sentMsgs
+        requires addReq.msg.seqNo in v.hosts[0].seqNoAssgn
+        requires multReq == v.hosts[0].seqNoAssgn[addReq.msg.seqNo]
+        requires latestResultIdx == |v.hosts[0].intermediateResults[multReq]| - 1
+        requires addReq.msg.seqNo == v.hosts[0].firstSeqNo[multReq] + latestResultIdx + 1
+        ensures addReq.msg == AddSvc.AddRequest(addReq.msg.seqNo, |v.hosts[0].intermediateResults[multReq]| * multReq.msg.y, multReq.msg.y)
+    {
+        if (|v.hosts[0].intermediateResults[multReq]| > 0) {
+            assert Inv_InductiveMultiplicationImpl(c, v, multReq);
+        }
+        assert Inv_AddRequestsImpl(c, v, addReq);
+    }
+
+    lemma Inv_AddRequestsHelper(c: Constants, v: Variables, v': Variables, msgOps: MessageOps, svcReply: Message<AddSvc.ServiceReply>, nextAddReq: Message<AddSvc.ServiceRequest>)
+        requires Next(c, v, v', msgOps)
+        requires Inv(c, v)
+        requires Host.ReceiveIntermediateResponseImpl(c.hosts[0], v.hosts[0], v'.hosts[0], msgOps, svcReply)
+        requires msgOps.send == { Message(nextAddReq.src, nextAddReq.dest, AddSvc.MarshallServiceRequest(nextAddReq.msg)) }
+        ensures nextAddReq.msg.seqNo in v'.hosts[0].seqNoAssgn
+        ensures Inv_AddRequests(c, v')
+    {
+        assert msgOps.send == {Message(c.hosts[0].idSelf, c.hosts[0].idAddSvc, AddSvc.MarshallServiceRequest(AddSvc.AddRequest(svcReply.msg.seqNo + 1, svcReply.msg.sum, v.hosts[0].seqNoAssgn[svcReply.msg.seqNo].msg.y)))};
+        AddSvc.MarshallParseInverse();
+        assert v.hosts[0].seqNoAssgn[svcReply.msg.seqNo] in v.hosts[0].firstSeqNo;
+        assert v.hosts[0].firstSeqNo[v.hosts[0].seqNoAssgn[svcReply.msg.seqNo]] <= svcReply.msg.seqNo < v.hosts[0].firstSeqNo[v.hosts[0].seqNoAssgn[svcReply.msg.seqNo]] + v.hosts[0].seqNoAssgn[svcReply.msg.seqNo].msg.x - 1;
+        assert nextAddReq.msg.seqNo == svcReply.msg.seqNo + 1;
+        assert nextAddReq.msg.seqNo in v'.hosts[0].seqNoAssgn;
+        assert Inv_AddRequestsImpl(c, v', nextAddReq);
+        assert v'.network.sentMsgs == v.network.sentMsgs + {Message(nextAddReq.src, nextAddReq.dest, AddSvc.MarshallServiceRequest(nextAddReq.msg))};
+        forall addReq: Message<AddSvc.ServiceRequest> | addReq.src == c.hosts[0].idSelf && Message(addReq.src, addReq.dest, AddSvc.MarshallServiceRequest(addReq.msg)) in v'.network.sentMsgs && addReq.msg.seqNo in v'.hosts[0].seqNoAssgn
+            ensures Inv_AddRequestsImpl(c, v', addReq)
+        {
+            if (addReq == nextAddReq) {
+
+            } else {
+                assert(Message(addReq.src, addReq.dest, AddSvc.MarshallServiceRequest(addReq.msg)) in v.network.sentMsgs);
+                assert(Inv_AddRequests(c, v));
+                assert(Inv_AddRequestsImpl(c, v, addReq));
+                assert Inv_AddRequestsImpl(c, v', addReq);
+            }
+        }
+    }
+
+    lemma Inv_InductiveMultiplicationHelper(c: Constants, v: Variables, v': Variables, msgOps: MessageOps, svcReply: Message<AddSvc.ServiceReply>, multReq: Message<Host.Spec.ServiceRequest>)
+        requires Next(c, v, v', msgOps)
+        requires Inv(c, v)
+        requires Host.ReceiveIntermediateResponseImpl(c.hosts[0], v.hosts[0], v'.hosts[0], msgOps, svcReply) || Host.ReceiveFinalResponseImpl(c.hosts[0], v.hosts[0], v'.hosts[0], msgOps, svcReply)
+        requires multReq == v'.hosts[0].seqNoAssgn[svcReply.msg.seqNo]
+        ensures Inv_InductiveMultiplicationImpl(c, v', multReq)
+    {
+        var seqNo := svcReply.msg.seqNo; 
+        var addReq := ApplyServiceCorrespondence(c, v, v', msgOps, svcReply);
+        assert Network.Next(c.network, v.network, v'.network, msgOps, 0);
+        assert svcReply.dest == 0;
+        assert svcReply.dest == addReq.src;
+        assert addReq.msg.seqNo == seqNo;
+        var latestResultIdx := |v.hosts[0].intermediateResults[multReq]| - 1;
+        assert seqNo == v.hosts[0].firstSeqNo[multReq] + latestResultIdx + 1;
+        ApplyInv_AddRequestsImpl(c, v, addReq, multReq, |v.hosts[0].intermediateResults[multReq]| - 1);
+        assert addReq == Message(addReq.src, addReq.dest, AddSvc.AddRequest(seqNo, |v.hosts[0].intermediateResults[multReq]| * multReq.msg.y, multReq.msg.y));
+        assert svcReply.msg.sum == |v.hosts[0].intermediateResults[multReq]| * multReq.msg.y + multReq.msg.y;
+        Inv_InductiveMultiplicationLemma(|v.hosts[0].intermediateResults[multReq]|, multReq.msg.y, svcReply.msg.sum);
+        assert svcReply.msg.sum == (|v.hosts[0].intermediateResults[multReq]| + 1) * multReq.msg.y;
 
         if (|v.hosts[0].intermediateResults[multReq]| > 0)
         {
-            assert InductiveMultiplication(c, v, multReq);
-            assert InductiveMultiplication(c, v', multReq);
+            assert Inv(c, v);
+            assert Inv_InductiveMultiplicationImpl(c, v, multReq);
+            assert Inv_InductiveMultiplicationImpl(c, v', multReq);
         }
         else 
         {
-            assert InductiveMultiplication(c, v', multReq);
+            assert Inv(c, v);
+            assert Inv_InductiveMultiplicationImpl(c, v', multReq);
         }
     }
 
@@ -107,57 +222,63 @@ module MultiplicationServiceComponent refines RefinementTheorem {
         assert Host.Next(c.hosts[0], v.hosts[0], v'.hosts[0], msgOps);
         if (Host.ReceiveRequest(c.hosts[0], v.hosts[0], v'.hosts[0], msgOps))
         {
+            assume false;
             var request :| Host.ReceiveRequestImpl(c.hosts[0], v.hosts[0], v'.hosts[0], msgOps, request);
-            assert msgOps.recv == {Host.Spec.MarshallServiceRequest(request)};
+            assert msgOps.recv == {Message(request.src, c.hosts[0].idSelf, Host.Spec.MarshallServiceRequest(request.msg))};
             ServiceRequestsAbstractionLemma(msgOps.recv);
             assert ServiceRequestsAbstraction(msgOps.recv) == {request};
-            var sent := AddSvc.MarshallServiceRequest(AddSvc.AddRequest(c.hosts[0].id, v.hosts[0].nextSeqNo, 0, request.y));
+            var sent := Message(c.hosts[0].idSelf, c.hosts[0].idAddSvc, AddSvc.MarshallServiceRequest(AddSvc.AddRequest(v.hosts[0].nextSeqNo, 0, request.msg.y)));
             AddSvc.MarshallParseInverse();
             assert msgOps.send == {sent};
             ServiceRepliesAbstractionLemma(msgOps.send);
-            UniqueParsingAxiom(sent);
+            UniqueParsingAxiom(sent.msg);
             assert Host.Spec.ReceiveRequest(ConstantsAbstraction(c), VariablesAbstraction(c, v), VariablesAbstraction(c, v'), ServiceRequestsAbstraction(msgOps.recv), ServiceRepliesAbstraction(msgOps.send));
         }
         else if (Host.ReceiveIntermediateResponse(c.hosts[0], v.hosts[0], v'.hosts[0], msgOps))
         {
             var svcReply :| Host.ReceiveIntermediateResponseImpl(c.hosts[0], v.hosts[0], v'.hosts[0], msgOps, svcReply);
-            var seqNo := svcReply.seqNo;
-            assert msgOps.recv == {AddSvc.MarshallServiceReply(svcReply)};
+            var seqNo := svcReply.msg.seqNo;
+            assert msgOps.recv == {Message(svcReply.src, svcReply.dest, AddSvc.MarshallServiceReply(svcReply.msg))};
             AddSvc.MarshallParseInverse();
             ServiceRequestsAbstractionLemma(msgOps.recv);
-            UniqueParsingAxiom(AddSvc.MarshallServiceReply(svcReply));
+            UniqueParsingAxiom(AddSvc.MarshallServiceReply(svcReply.msg));
             assert ServiceRequestsAbstraction(msgOps.recv) == {};
-            var sent := AddSvc.MarshallServiceRequest(AddSvc.AddRequest(c.hosts[0].id, seqNo + 1, svcReply.sum, v.hosts[0].seqNoAssgn[seqNo].y));
+            var sent := Message(c.hosts[0].idSelf, c.hosts[0].idAddSvc, AddSvc.MarshallServiceRequest(AddSvc.AddRequest(seqNo + 1, svcReply.msg.sum, v.hosts[0].seqNoAssgn[seqNo].msg.y)));
             assert msgOps.send == {sent};
             AddSvc.MarshallParseInverse();
             ServiceRepliesAbstractionLemma(msgOps.send);
-            UniqueParsingAxiom(sent);
+            UniqueParsingAxiom(sent.msg);
             assert ServiceRepliesAbstraction(msgOps.recv) == {};
             assert VariablesAbstraction(c, v) == VariablesAbstraction(c, v') && ServiceRequestsAbstraction(msgOps.recv) == {} && ServiceRepliesAbstraction(msgOps.send) == {};
 
-            InvHelper(c, v, v', msgOps, svcReply);
+            Inv_AddRequestsHelper(c, v, v', msgOps, svcReply, Message(c.hosts[0].idSelf, c.hosts[0].idAddSvc, AddSvc.AddRequest(seqNo + 1, svcReply.msg.sum, v.hosts[0].seqNoAssgn[seqNo].msg.y)));
+            assume false;
+            var multReq := v'.hosts[0].seqNoAssgn[svcReply.msg.seqNo];
+            Inv_InductiveMultiplicationHelper(c, v, v', msgOps, svcReply, multReq);
         }
         else {
+            assume false;
             var svcReply :| Host.ReceiveFinalResponseImpl(c.hosts[0], v.hosts[0], v'.hosts[0], msgOps, svcReply);
-            assert msgOps.recv == {AddSvc.MarshallServiceReply(svcReply)};
+            assert msgOps.recv == {Message(svcReply.src, svcReply.dest, AddSvc.MarshallServiceReply(svcReply.msg))};
             AddSvc.MarshallParseInverse();
             ServiceRequestsAbstractionLemma(msgOps.recv);
-            UniqueParsingAxiom(AddSvc.MarshallServiceReply(svcReply));
+            UniqueParsingAxiom(AddSvc.MarshallServiceReply(svcReply.msg));
             assert ServiceRequestsAbstraction(msgOps.recv) == {};
-            var absReply := Host.Spec.MultiplyReply(v.hosts[0].seqNoAssgn[svcReply.seqNo].clientId, v.hosts[0].seqNoAssgn[svcReply.seqNo].seqNo, svcReply.sum);
-            var sent := Host.Spec.MarshallServiceReply(absReply);
+            var absReply := Message(c.hosts[0].idSelf, v.hosts[0].seqNoAssgn[svcReply.msg.seqNo].src, Host.Spec.MultiplyReply(v.hosts[0].seqNoAssgn[svcReply.msg.seqNo].msg.seqNo, svcReply.msg.sum));
+            var sent := Message(absReply.src, absReply.dest, Host.Spec.MarshallServiceReply(absReply.msg));
             assert msgOps.send == {sent};
             ServiceRepliesAbstractionLemma(msgOps.send);
             assert ServiceRepliesAbstraction(msgOps.send) == {absReply};
 
-            InvHelper(c, v, v', msgOps, svcReply);
+            var multReq := v'.hosts[0].seqNoAssgn[svcReply.msg.seqNo];
+            Inv_InductiveMultiplicationHelper(c, v, v', msgOps, svcReply, multReq);
 
-            assert InductiveMultiplication(c, v', v'.hosts[0].seqNoAssgn[svcReply.seqNo]);
-            assert absReply.product == v.hosts[0].seqNoAssgn[svcReply.seqNo].x * v.hosts[0].seqNoAssgn[svcReply.seqNo].y;
-            assert absReply.clientId == v.hosts[0].seqNoAssgn[svcReply.seqNo].clientId;
-            assert absReply.seqNo == v.hosts[0].seqNoAssgn[svcReply.seqNo].seqNo;
-            assert v.hosts[0].seqNoAssgn[svcReply.seqNo] in v.hosts[0].requests;
-            assert v.hosts[0].seqNoAssgn[svcReply.seqNo] in VariablesAbstraction(c, v).requests;
+            assert Inv_InductiveMultiplicationImpl(c, v', v'.hosts[0].seqNoAssgn[svcReply.msg.seqNo]);
+            assert absReply.msg.product == v.hosts[0].seqNoAssgn[svcReply.msg.seqNo].msg.x * v.hosts[0].seqNoAssgn[svcReply.msg.seqNo].msg.y;
+            assert absReply.dest == v.hosts[0].seqNoAssgn[svcReply.msg.seqNo].src;
+            assert absReply.msg.seqNo == v.hosts[0].seqNoAssgn[svcReply.msg.seqNo].msg.seqNo;
+            assert v.hosts[0].seqNoAssgn[svcReply.msg.seqNo] in v.hosts[0].requests;
+            assert v.hosts[0].seqNoAssgn[svcReply.msg.seqNo] in VariablesAbstraction(c, v).requests;
             assert Host.Spec.SendResponse(ConstantsAbstraction(c), VariablesAbstraction(c, v), VariablesAbstraction(c, v'), ServiceRequestsAbstraction(msgOps.recv), ServiceRepliesAbstraction(msgOps.send));
         }
     }
