working/composition/event_based_refinement/load_balancer/service_correspondence/multiplication_service/MultiplicationServiceSpec.t.dfy
@@ -3,17 +3,17 @@ include "../shared/AbstractServiceSpec.t.dfy"
 module MultiplicationServiceSpec refines AbstractServiceSpec {
     datatype Constants = Constants
 
-    datatype ServiceRequest = MultiplyRequest(clientId: ClientId, seqNo: SeqNo, x: int, y: int)
-    datatype ServiceReply = MultiplyReply(clientId: ClientId, seqNo: SeqNo, product: int)
+    datatype ServiceRequest = MultiplyRequest(seqNo: SeqNo, x: int, y: int)
+    datatype ServiceReply = MultiplyReply(seqNo: SeqNo, product: int)
 
-    datatype Variables = Variables(requests: set<ServiceRequest>, replies: set<ServiceReply>)
+    datatype Variables = Variables(requests: set<Message<ServiceRequest>>, replies: set<Message<ServiceReply>>)
 
     ghost predicate Init(c: Constants, v: Variables) {
         && |v.requests| == 0
         && |v.replies| == 0
     }
 
-    ghost predicate ReceiveRequest(c: Constants, v: Variables, v': Variables, requests: set<ServiceRequest>, replies: set<ServiceReply>) {
+    ghost predicate ReceiveRequest(c: Constants, v: Variables, v': Variables, requests: set<Message<ServiceRequest>>, replies: set<Message<ServiceReply>>) {
         exists request ::
             && requests == {request} 
             && replies == {}
@@ -21,17 +21,18 @@ module MultiplicationServiceSpec refines AbstractServiceSpec {
             && v'.replies == v.replies
     }
 
-    ghost predicate SendResponse(c: Constants, v: Variables, v': Variables, requests: set<ServiceRequest>, replies: set<ServiceReply>) {
+    ghost predicate SendResponse(c: Constants, v: Variables, v': Variables, requests: set<Message<ServiceRequest>>, replies: set<Message<ServiceReply>>) {
         exists request, reply ::
             && requests == {} 
             && replies == {reply}
             && v'.requests == v.requests
             && request in v.requests
             && v'.replies == v.replies + {reply}
-            && reply == MultiplyReply(request.clientId, request.seqNo, request.x * request.y)
+            && reply.msg == MultiplyReply(request.msg.seqNo, request.msg.x * request.msg.y)
+            && reply.dest == request.src
     }
 
-    ghost predicate Next(c: Constants, v: Variables, v': Variables, requests: set<ServiceRequest>, replies: set<ServiceReply>) {
+    ghost predicate Next(c: Constants, v: Variables, v': Variables, requests: set<Message<ServiceRequest>>, replies: set<Message<ServiceReply>>) {
         || ReceiveRequest(c, v, v', requests, replies)
         || SendResponse(c, v, v', requests, replies)
     }
