working/composition/event_based_refinement/load_balancer/service_correspondence/shared/AbstractNetwork.t.dfy
@@ -1,7 +1,6 @@
 include "Types.t.dfy"
 include "AbstractHost.t.dfy"
 
-// copied from chapter 5 exercise 1
 abstract module AbstractNetwork {
   import opened Types
   import opened Host : AbstractHost
@@ -10,20 +9,22 @@ abstract module AbstractNetwork {
 
   // Network state is the set of messages ever sent. Once sent, we'll
   // allow it to be delivered over and over.
-  // (We don't have packet headers, so duplication, besides being realistic,
-  // also doubles as how multiple parties can hear the message.)
-  datatype Variables = Variables(sentMsgs:set<seq<byte>>)
+  datatype Variables = Variables(sentMsgs:set<Message<seq<byte>>>)
 
   ghost predicate Init(c: Constants, v: Variables)
   {
     && v.sentMsgs == {}
   }
 
-  ghost predicate Next(c: Constants, v: Variables, v': Variables, msgOps: MessageOps)
+  ghost predicate Next(c: Constants, v: Variables, v': Variables, msgOps: MessageOps, hostId: nat)
   {
     // Only allow receipt of a message if we've seen it has been sent.
     && (forall m :: m in msgOps.recv ==> m in v.sentMsgs)
     // Record the sent message, if there was one.
     && v'.sentMsgs == v.sentMsgs + msgOps.send
+    // only allow received messages on given host
+    && (forall recv_msg :: recv_msg in msgOps.recv ==> recv_msg.dest == hostId)
+    // only allow sent messages from given host
+    && (forall send_msg :: send_msg in msgOps.send ==> send_msg.src == hostId)
   }
 }
